theories/sim/program.v
@@ -31,7 +31,7 @@ Proof.
     intros. simpl. exists 1%nat.
     apply (sim_body_result _ _ _ _ (ValR vs) (ValR vt)).
     intros VALID.
-    have ?: vrel_expr (init_res ⋅ r') (of_result #vs) (of_result #vt).
+    have ?: vrel_res (init_res ⋅ r') (#vs) (#vt).
     { do 2 eexists. do 2 (split; [done|]).
       eapply vrel_mono; [done|apply cmra_included_r|done]. }
     split; last split; [..|done].
